TSO prom: define all steps
- define read, write, rmw
- remove the case of store forwarding
- remove annotation of state & local
- remove order (rel & acq)
- remove eqts

Signed-off-by: Kyeongmin Cho <kyeongmin.cho@kaist.ac.kr>

src/promising/TsoPromising.v
@@ -20,221 +20,81 @@ Require Import PromisingArch.promising.CommonPromising.
 Set Implicit Arguments.
 
 
-Module FwdItem.
-Section FwdItem.
-  Context `{A: Type, _: orderC A eq}.
-
-  Inductive t := mk {
-    ts: Time.t;
-    view: View.t (A:=A);
-    ex: bool;
-  }.
-  Hint Constructors t.
-
-  Definition init: t := mk bot bot false.
-
-  Definition read_view (fwd:t) (tsx:Time.t) (ord:OrdR.t): View.t (A:=A) :=
-    if andb (fwd.(ts) == tsx) (negb (andb fwd.(ex) (OrdR.ge ord OrdR.acquire_pc)))
-    then fwd.(view)
-    else View.mk tsx bot.
-End FwdItem.
-End FwdItem.
-
-Section Eqts.
-  Context `{A: Type, B: Type, _: orderC A eq, _: orderC B eq}.
-
-  Inductive eqts_view (v1: View.t (A:=A)) (v2: View.t (A:=B)): Prop :=
-  | eqts_view_intro
-      (TS: v1.(View.ts) = v2.(View.ts))
-  .
-  Hint Constructors eqts_view.
-
-  Inductive eqts_fwd (fwd1:FwdItem.t (A:=A)) (fwd2:FwdItem.t (A:=B)): Prop :=
-  | eqts_fwd_intro
-      (TS: fwd1.(FwdItem.ts) = fwd2.(FwdItem.ts))
-      (VIEW: eqts_view fwd1.(FwdItem.view) fwd2.(FwdItem.view))
-      (EX: fwd1.(FwdItem.ex) = fwd2.(FwdItem.ex))
-  .
-  Hint Constructors eqts_fwd.
-
-  Inductive eqts_val (v1:ValA.t (A:=View.t (A:=A))) (v2:ValA.t (A:=View.t (A:=B))): Prop :=
-  | eqts_val_intro
-      (VAL: v1.(ValA.val) = v2.(ValA.val))
-      (VIEW: eqts_view v1.(ValA.annot) v2.(ValA.annot))
-  .
-  Hint Constructors eqts_val.
-
-  Inductive eqts_event: forall (e1:Event.t (A:=View.t (A:=A))) (e2:Event.t (A:=View.t (A:=B))), Prop :=
-  | eqts_event_internal:
-      eqts_event Event.internal Event.internal
-  | eqts_event_read
-      ex rmw_fail ord vloc1 vloc2 res1 res2
-      (VLOC: eqts_val vloc1 vloc2)
-      (RES: eqts_val res1 res2):
-      eqts_event (Event.read ex rmw_fail ord vloc1 res1) (Event.read ex rmw_fail ord vloc2 res2)
-  | eqts_event_write
-      ex ord vloc1 vloc2 vval1 vval2 res1 res2
-      (VLOC: eqts_val vloc1 vloc2)
-      (VVAL: eqts_val vval1 vval2)
-      (RES: eqts_val res1 res2):
-      eqts_event (Event.write ex ord vloc1 vval1 res1) (Event.write ex ord vloc2 vval2 res2)
-  | eqts_event_rmw
-      ordr ordw vloc1 vloc2 old1 old2 new1 new2:
-      eqts_event (Event.rmw ordr ordw vloc1 old1 new1) (Event.rmw ordr ordw vloc2 old2 new2)
-  | eqts_event_barrier
-      b:
-      eqts_event (Event.barrier b) (Event.barrier b)
-  | eqts_event_control
-      ctrl1 ctrl2
-      (CTRL: eqts_view ctrl1 ctrl2):
-      eqts_event (Event.control ctrl1) (Event.control ctrl2)
-  .
-  Hint Constructors eqts_event.
-End Eqts.
-
-Section EqtsEquiv.
-  Context `{A: Type, _: orderC A eq}.
-
-  Global Program Instance eqts_view_equiv: Equivalence (@eqts_view A A).
-  Next Obligation. econs. ss. Qed.
-  Next Obligation. econs. inv H1. ss. Qed.
-  Next Obligation. econs. inv H1. inv H2. etrans; eauto. Qed.
-
-  Global Program Instance eqts_fwd_equiv: Equivalence (@eqts_fwd A A).
-  Next Obligation. econs; ss. Qed.
-  Next Obligation. ii. destruct x, y. inv H1. ss. subst. econs; ss. symmetry. ss. Qed.
-  Next Obligation. ii. destruct x, y, z. inv H1. inv H2. ss. subst. econs; ss. etrans; eauto. Qed.
-
-  Global Program Instance eqts_val_equiv: Equivalence eqts_val.
-  Next Obligation. econs; ss. Qed.
-  Next Obligation. ii. destruct x, y. inv H1. ss. subst. econs; ss. symmetry. ss. Qed.
-  Next Obligation. ii. destruct x, y, z. inv H1. inv H2. ss. subst. econs; ss. etrans; eauto. Qed.
-
-  Global Program Instance eqts_event_equiv: Equivalence eqts_event.
-  Next Obligation. ii. destruct x; econs; ss. Qed.
-  Next Obligation.
-    ii. inv H1; econs; ss.
-    all: symmetry; ss.
-  Qed.
-  Next Obligation.
-    ii. inv H1; inv H2; econs; ss.
-    all: etrans; eauto.
-  Qed.
-End EqtsEquiv.
-
 Module Local.
 Section Local.
-  Context `{A: Type, _: orderC A eq}.
-
   Inductive t := mk {
-    coh: Loc.t -> View.t (A:=A);
-    vrn: View.t (A:=A);
-    vwn: View.t (A:=A);
-    vro: View.t (A:=A);
-    vwo: View.t (A:=A);
-    vrel: View.t (A:=A);
-    fwdbank: Loc.t -> (FwdItem.t (A:=A));
+    coh: Loc.t -> View.t (A:=unit);
+    vrn: View.t (A:=unit);
+    vwn: View.t (A:=unit);
+    vro: View.t (A:=unit);
+    vwo: View.t (A:=unit);
   }.
   Hint Constructors t.
 
-  Definition init: t := mk bot bot bot bot bot bot (fun _ => FwdItem.init).
+  Definition init: t := mk bot bot bot bot bot.
 
-  Inductive read (ex:bool) (ord:OrdR.t) (vloc res:ValA.t (A:=View.t (A:=A))) (ts:Time.t) (lc1:t) (mem1: Memory.t) (lc2:t): Prop :=
+  Inductive read (vloc res:ValA.t (A:=unit)) (ts:Time.t) (lc1:t) (mem1: Memory.t) (lc2:t): Prop :=
   | read_intro
-      loc val view
+      loc val
       view_pre view_msg view_post
       (LOC: loc = vloc.(ValA.val))
-      (VIEW: view = vloc.(ValA.annot))
-      (VIEW_PRE: view_pre = joins [view; lc1.(vrn); (ifc (OrdR.ge ord OrdR.acquire) lc1.(vrel))])
+      (VIEW_PRE: view_pre = lc1.(vrn))
       (COH: Memory.latest loc ts (lc1.(coh) loc).(View.ts) mem1)
       (LATEST: Memory.latest loc ts view_pre.(View.ts) mem1)
       (MSG: Memory.read loc ts mem1 = Some val)
-      (VIEW_MSG: view_msg = FwdItem.read_view (lc1.(fwdbank) loc) ts ord)
+      (VIEW_MSG: view_msg = View.mk ts bot)
       (VIEW_POST: view_post = join view_pre view_msg)
-      (RES: res = ValA.mk _ val view_post)
+      (RES: res = ValA.mk _ val bot)
       (LC2: lc2 =
             mk
               (fun_add loc (join (lc1.(coh) loc) view_post) lc1.(coh))
-              (join lc1.(vrn) (ifc (OrdR.ge ord OrdR.acquire_pc) view_post))
-              (join lc1.(vwn) (ifc (OrdR.ge ord OrdR.acquire_pc) view_post))
+              (join lc1.(vrn) view_post)
+              (join lc1.(vwn) view_post)
               (join lc1.(vro) view_post)
-              lc1.(vwo)
-              lc1.(vrel)
-              lc1.(fwdbank))
+              lc1.(vwo))
   .
   Hint Constructors read.
 
-  Inductive write (ex:bool) (ord:OrdW.t) (vloc vval res:ValA.t (A:=View.t (A:=A))) (ts:Time.t) (tid:Id.t) (view_pre:View.t (A:=A)) (lc1:t) (mem1: Memory.t) (lc2:t) (mem2: Memory.t): Prop :=
+  Inductive write (vloc vval res:ValA.t (A:=unit)) (ts:Time.t) (tid:Id.t) (lc1:t) (mem1: Memory.t) (lc2:t) (mem2: Memory.t): Prop :=
   | write_intro
       loc val
       view_loc view_val
+      view_post
       (LOC: loc = vloc.(ValA.val))
       (VIEW_LOC: view_loc = vloc.(ValA.annot))
       (VAL: val = vval.(ValA.val))
       (VIEW_VAL: view_val = vval.(ValA.annot))
+      (VIEW_POST: view_post = View.mk ts bot)
       (MEM: Memory.append (Msg.mk loc val tid) mem1 = (ts, mem2))
-      (RES: res = ValA.mk _ 0 (View.mk bot view_pre.(View.annot)))
+      (RES: res = ValA.mk _ 0 bot)
       (LC2: lc2 =
             mk
-              (fun_add loc (View.mk ts bot) lc1.(coh))
+              (fun_add loc view_post lc1.(coh))
               lc1.(vrn)
-              lc1.(vwn)
+              (join lc1.(vwn) view_post)
               lc1.(vro)
-              (join lc1.(vwo) (View.mk ts bot))
-              (join lc1.(vrel) (View.mk (ifc (OrdW.ge ord OrdW.release) ts) bot))
-              (fun_add loc (FwdItem.mk ts (join view_loc view_val) ex) lc1.(fwdbank)))
+              (join lc1.(vwo) view_post))
   .
   Hint Constructors write.
 
-  (* writable *)
-      (* (EX: ex -> exists eb, *)
-      (*      <<TSX: lc1.(exbank) = Some eb>> /\ *)
-      (*      <<EX: eb.(Exbank.loc) = loc -> Memory.exclusive tid loc eb.(Exbank.ts) ts mem1>>) *)
-
-  Inductive rmw (ordr:OrdR.t) (ordw:OrdW.t) (vloc vold vnew:ValA.t (A:=View.t (A:=A))) (ts:Time.t) (tid:Id.t) (view_pre:View.t (A:=A)) (lc1:t) (mem1: Memory.t) (lc2:t) (mem2: Memory.t): Prop :=
+  Inductive rmw (vloc vold vnew:ValA.t (A:=unit)) (ts:Time.t) (tid:Id.t) (lc1:t) (mem1:Memory.t) (lc2:t) (mem2:Memory.t): Prop :=
   | rmw_intro
-      loc val prev_ts prev_val (* CHECK: 파라미터로 prev_ts가 필요하지 않은가? *)
-      view_loc view_val
+      loc old new old_ts
       view_post
       (LOC: loc = vloc.(ValA.val))
-      (VIEW: view_loc = vloc.(ValA.annot))
-
-      (* pre = addr \/ rnew \/ (rk >= acq ? ts.rel) *)
-      (VIEW_PRE: view_pre = joins [view_loc; lc1.(vrn); (ifc (OrdR.ge ordr OrdR.acquire) lc1.(vrel))])
-
-      (* writable *)
-      (COH: lt (lc1.(coh) loc).(View.ts) ts)
-      (EXT: lt view_pre.(View.ts) ts)
-
-      (* forall t', prev_t < t' <= t --> M(t').loc != l *)
-      (LATEST: Memory.latest loc prev_ts ts mem1)
-
-      (* CHECK: read(M,l,prev_t) = v = vold ? *)
-      (MSG: Memory.read loc prev_ts mem1 = Some prev_val)
-      (OLD: vold.(ValA.val) = prev_val)
-
-      (* CHECK: post = t ? *)
-      (VIEW_POST: view_post = (View.mk ts bot))
-
-      (* [e2] = v@data *)
-      (VAL: val = vnew.(ValA.val))
-      (VIEW_VAL: view_val = vnew.(ValA.annot))
-
-      (MEM: Memory.append (Msg.mk loc val tid) mem1 = (ts, mem2))
-
-      (* CHECK: regs view는 사라지는 것? *)
-      (* (RES: res = ValA.mk _ 0 (View.mk bot view_pre.(View.annot))) *)
-
-      (LC2: lc2 =
+      (LATEST: Memory.latest loc old_ts ts mem1)
+      (MSG: Memory.read loc old_ts mem1 = Some old)
+      (OLD: vold.(ValA.val) = old)
+      (NEW: new = vnew.(ValA.val))
+      (VIEW_POST: view_post = View.mk ts bot)
+      (MEM: Memory.append (Msg.mk loc new tid) mem1 = (ts, mem2))
+      (LC: lc2 =
             mk
-              (fun_add loc view_post lc1.(coh)) (* read *)
-              (join lc1.(vrn) (ifc (OrdR.ge ordr OrdR.acquire_pc) view_post)) (* read *)
-              (join lc1.(vwn) (ifc (OrdR.ge ordr OrdR.acquire_pc) view_post)) (* read *)
-              (join lc1.(vro) view_post) (* read *)
-              (join lc1.(vwo) view_post) (* write *)
-              (join lc1.(vrel) ((ifc (OrdW.ge ordw OrdW.release) view_post))) (* write *)
-              (* CHECK: addr view와 data view가 둘 다 필요한가? *)
-              (fun_add loc (FwdItem.mk ts (join view_loc view_val) false) lc1.(fwdbank))) (* write *)
+              (fun_add loc view_post lc1.(coh))
+              (join lc1.(vrn) view_post)
+              (join lc1.(vwn) view_post)
+              (join lc1.(vro) view_post)
+              (join lc1.(vwo) view_post))
   .
   Hint Constructors rmw.
 
@@ -247,13 +107,11 @@ Section Local.
               (joins [lc1.(vrn); ifc rr lc1.(vro); ifc wr lc1.(vwo)])
               (joins [lc1.(vwn); ifc rw lc1.(vro); ifc ww lc1.(vwo)])
               lc1.(vro)
-              lc1.(vwo)
-              lc1.(vrel)
-              lc1.(fwdbank))
+              lc1.(vwo))
   .
   Hint Constructors dmb.
 
-  Inductive step (event:Event.t (A:=View.t (A:=A))) (tid:Id.t) (mem1 mem2:Memory.t) (lc1 lc2:t): Prop :=
+  Inductive step (event:Event.t (A:=unit)) (tid:Id.t) (mem1 mem2:Memory.t) (lc1 lc2:t): Prop :=
   | step_internal
       (EVENT: event = Event.internal)
       (LC: lc2 = lc1)
@@ -261,16 +119,16 @@ Section Local.
   | step_read
       ord vloc res ts
       (EVENT: event = Event.read false false ord vloc res)
-      (STEP: read false ord vloc res ts lc1 mem1 lc2)
+      (STEP: read vloc res ts lc1 mem1 lc2)
       (MEM: mem2 = mem1)
   | step_write
-      ord vloc vval res ts view_pre
+      ord vloc vval res ts
       (EVENT: event = Event.write false ord vloc vval res)
-      (STEP: write false ord vloc vval res ts tid view_pre lc1 mem1 lc2 mem2)
+      (STEP: write vloc vval res ts tid lc1 mem1 lc2 mem2)
   | step_rmw
-      ordr ordw vloc vold vnew ts view_pre
+      ordr ordw vloc vold vnew ts
       (EVENT: event = Event.rmw ordr ordw vloc vold vnew)
-      (STEP: rmw ordr ordw vloc vold vnew ts tid view_pre lc1 mem1 lc2 mem2)
+      (STEP: rmw vloc vold vnew ts tid lc1 mem1 lc2 mem2)
   | step_dmb (* TODO: check it *)
       rr rw wr ww
       (EVENT: event = Event.barrier (Barrier.dmb rr rw wr ww))
@@ -279,13 +137,6 @@ Section Local.
   .
   Hint Constructors step.
 
-  Inductive wf_fwdbank (loc:Loc.t) (mem:Memory.t) (coh: Time.t) (fwd:FwdItem.t (A:=A)): Prop :=
-  | wf_fwdbank_intro
-      (TS: fwd.(FwdItem.ts) <= Memory.latest_ts loc coh mem)
-      (VIEW: fwd.(FwdItem.view).(View.ts) <= fwd.(FwdItem.ts))
-      (VAL: exists val, Memory.read loc fwd.(FwdItem.ts) mem = Some val)
-  .
-
   Inductive wf (tid:Id.t) (mem:Memory.t) (lc:t): Prop :=
   | wf_intro
       (COH: forall loc, (lc.(coh) loc).(View.ts) <= List.length mem)
@@ -293,78 +144,42 @@ Section Local.
       (VWN: lc.(vwn).(View.ts) <= List.length mem)
       (VRO: lc.(vro).(View.ts) <= List.length mem)
       (VWO: lc.(vwo).(View.ts) <= List.length mem)
-      (VREL: lc.(vrel).(View.ts) <= List.length mem)
-      (FWDBANK: forall loc, wf_fwdbank loc mem (lc.(coh) loc).(View.ts) (lc.(fwdbank) loc))
   .
   Hint Constructors wf.
 
   Lemma init_wf tid: wf tid Memory.empty init.
   Proof.
     econs; ss; i; try by apply bot_spec.
-    - econs; ss. eexists. ss.
-  Qed.
-
-  (* CHECK: 원래 주석처리 되어있었음 *)
-  (* Lemma fwd_read_view_coh_le *)
-  (*       tid mem lc *)
-  (*       (WF: wf tid mem lc) *)
-  (*       loc ord ts *)
-  (*       (COH: (lc.(coh) loc).(View.ts) <= ts): *)
-  (*   ((lc.(Local.fwdbank) loc).(FwdItem.read_view) ts ord).(View.ts) <= ts. *)
-  (* Proof. *)
-  (*   inv WF. exploit FWDBANK; eauto. i. des. *)
-  (*   unfold FwdItem.read_view. condtac; ss. etrans; eauto. etrans; eauto. *)
-  (* Qed. *)
-
-  Lemma fwd_view_le
-        tid mem lc loc ts ord
-        (WF: wf tid mem lc)
-        (COH: Memory.latest loc ts (lc.(coh) loc).(View.ts) mem):
-    (lc.(fwdbank) loc).(FwdItem.view).(View.ts) <=
-    (FwdItem.read_view (lc.(fwdbank) loc) ts ord).(View.ts).
-  Proof.
-    unfold FwdItem.read_view. condtac; ss.
-    inv WF. exploit FWDBANK. intro Y. inv Y.
-    rewrite VIEW, TS. apply Memory.latest_latest_ts. ss.
-  Qed.
-
-  Lemma fwd_read_view_le
-        tid mem lc loc ts ord
-        (WF: wf tid mem lc)
-        (COH: Memory.latest loc ts (lc.(coh) loc).(View.ts) mem):
-    (FwdItem.read_view (lc.(fwdbank) loc) ts ord).(View.ts) <= ts.
-  Proof.
-    inv WF. destruct (FWDBANK loc). des.
-    unfold FwdItem.read_view. condtac; ss.
-    destruct (equiv_dec (FwdItem.ts (fwdbank lc loc)) ts); ss. inv e. ss.
   Qed.
 
   Lemma read_spec
-        tid mem ex ord vloc res ts lc1 lc2
+        tid mem vloc res ts lc1 lc2
         (WF: Local.wf tid mem lc1)
-        (READ: Local.read ex ord vloc res ts lc1 mem lc2):
-    <<LATEST: Memory.latest vloc.(ValA.val) ts res.(ValA.annot).(View.ts) mem>> /\
+        (READ: Local.read vloc res ts lc1 mem lc2):
+    <<LATEST: Memory.latest vloc.(ValA.val) ts (length mem) mem>> /\
     <<COH: ts = Memory.latest_ts vloc.(ValA.val) (lc2.(Local.coh) vloc.(ValA.val)).(View.ts) mem>>.
   Proof.
     inv READ. ss. rewrite fun_add_spec. condtac; [|congr]. splits.
-    - apply Memory.latest_join; auto.
-      apply Memory.ge_latest. eapply fwd_read_view_le; eauto.
-    - unfold join. ss. apply le_antisym.
-      + unfold FwdItem.read_view. des_ifs.
-        * rewrite Bool.andb_true_iff in Heq. des.
-          destruct (equiv_dec (FwdItem.ts (fwdbank lc1 (ValA.val vloc))) ts); ss.
-          inv e0. inv WF. exploit FWDBANK. intro Y. inv Y.
-          eapply Memory.latest_ts_read_le; eauto.
-          rewrite TS, Memory.latest_latest_ts.
-          { apply join_l. }
-          { apply Memory.ge_latest. ss. }
-        * eapply Memory.latest_ts_read_le; eauto.
-          ss. repeat rewrite <- join_r. auto.
-      + hexploit fwd_read_view_le; eauto. i.
-        apply Memory.latest_latest_ts.
-        apply Memory.latest_join; ss.
-        apply Memory.latest_join; ss.
-        apply Memory.ge_latest. etrans; eauto.
+    - admit.
+    - admit.
+    (* - apply Memory.latest_join; auto. *)
+    (*   apply Memory.ge_latest. eapply fwd_read_view_le; eauto. *)
+    (* - unfold join. ss. apply le_antisym. *)
+    (*   + unfold FwdItem.read_view. des_ifs. *)
+    (*     * rewrite Bool.andb_true_iff in Heq. des. *)
+    (*       destruct (equiv_dec (FwdItem.ts (fwdbank lc1 (ValA.val vloc))) ts); ss. *)
+    (*       inv e0. inv WF. exploit FWDBANK. intro Y. inv Y. *)
+    (*       eapply Memory.latest_ts_read_le; eauto. *)
+    (*       rewrite TS, Memory.latest_latest_ts. *)
+    (*       { apply join_l. } *)
+    (*       { apply Memory.ge_latest. ss. } *)
+    (*     * eapply Memory.latest_ts_read_le; eauto. *)
+    (*       ss. repeat rewrite <- join_r. auto. *)
+    (*   + hexploit fwd_read_view_le; eauto. i. *)
+    (*     apply Memory.latest_latest_ts. *)
+    (*     apply Memory.latest_join; ss. *)
+    (*     apply Memory.latest_join; ss. *)
+    (*     apply Memory.ge_latest. etrans; eauto. *)
   Qed.
 
   Lemma interference_wf
@@ -377,9 +192,6 @@ Section Local.
     all: try rewrite app_length.
     all: try lia.
     - rewrite COH. lia.
-    - destruct (FWDBANK loc). des. econs; esplits; eauto.
-      + rewrite TS, Memory.latest_ts_append. ss.
-      + apply Memory.read_mon. eauto.
   Qed.
 
   Inductive le (lhs rhs:t): Prop :=
@@ -389,17 +201,16 @@ Section Local.
       (VWN: Order.le lhs.(vwn).(View.ts) rhs.(vwn).(View.ts))
       (VRO: Order.le lhs.(vro).(View.ts) rhs.(vro).(View.ts))
       (VWO: Order.le lhs.(vwo).(View.ts) rhs.(vwo).(View.ts))
-      (VREL: Order.le lhs.(vrel).(View.ts) rhs.(vrel).(View.ts))
   .
 
   (* CHECK: move? *)
   Global Program Instance le_partial_order: PreOrder le.
   Next Obligation. econs; refl. Qed.
-  Next Obligation. ii. inv H1. inv H2. econs; etrans; eauto. Qed.
+  Next Obligation. ii. inv H. inv H0. econs; etrans; eauto. Qed.
 
   Lemma read_incr
-        ex ord vloc res ts lc1 mem1 lc2
-        (LC: read ex ord vloc res ts lc1 mem1 lc2):
+        vloc res ts lc1 mem1 lc2
+        (LC: read vloc res ts lc1 mem1 lc2):
     le lc1 lc2.
   Proof.
     inv LC. econs; ss; try refl; try apply join_l.
@@ -408,8 +219,8 @@ Section Local.
   Qed.
 
   Lemma write_incr
-        ex ord vloc vval res ts tid view_pre lc1 mem1 lc2 mem2
-        (LC: write ex ord vloc vval res ts tid view_pre lc1 mem1 lc2 mem2):
+        vloc vval res ts tid lc1 mem1 lc2 mem2
+        (LC: write vloc vval res ts tid lc1 mem1 lc2 mem2):
     le lc1 lc2.
   Proof.
     inv LC. econs; ss; try refl; try apply join_l.
@@ -419,10 +230,9 @@ Section Local.
     admit.
   Qed.
 
-  (* TODO *)
   Lemma rmw_incr
-        ordr ordw vloc vold vnew ts tid view_pre lc1 mem1 lc2 mem2
-        (LC: rmw ordr ordw vloc vold vnew ts tid view_pre lc1 mem1 lc2 mem2):
+        vloc vold vnew ts tid lc1 mem1 lc2 mem2
+        (LC: rmw vloc vold vnew ts tid lc1 mem1 lc2 mem2):
     le lc1 lc2.
   Proof.
     inv LC. econs; ss; try refl; try apply join_l.
@@ -472,16 +282,14 @@ Ltac viewtac :=
 
 Module ExecUnit.
 Section ExecUnit.
-  Context `{A: Type, _: orderC A eq}.
-
   Inductive t := mk {
-    state: State.t (A:=View.t (A:=A));
-    local: Local.t (A:=A);
+    state: State.t (A:=unit);
+    local: Local.t;
     mem: Memory.t;
   }.
   Hint Constructors t.
 
-  Inductive step0 (tid:Id.t) (e1 e2:Event.t (A:=View.t (A:=A))) (eu1 eu2:t): Prop :=
+  Inductive step0 (tid:Id.t) (e1 e2:Event.t (A:=unit)) (eu1 eu2:t): Prop :=
   | step0_intro
       (STATE: State.step e1 eu1.(state) eu2.(state))
       (LOCAL: Local.step e2 tid eu1.(mem) eu2.(mem) eu1.(local) eu2.(local))
@@ -496,92 +304,47 @@ Section ExecUnit.
   .
   Hint Constructors step.
 
-  Inductive rmap_wf (mem:Memory.t) (rmap:RMap.t (A:=View.t (A:=A))): Prop :=
-  | rmap_wf_intro
-      (RMAP: forall r, (RMap.find r rmap).(ValA.annot).(View.ts) <= List.length mem)
-  .
-  Hint Constructors rmap_wf.
-
   Inductive wf (tid:Id.t) (eu:t): Prop :=
   | wf_intro
-      (STATE: rmap_wf eu.(mem) eu.(state).(State.rmap))
       (LOCAL: Local.wf tid eu.(mem) eu.(local))
   .
   Hint Constructors wf.
 
-  Lemma rmap_add_wf
-        mem rmap loc (val:ValA.t (A:=View.t (A:=A)))
-        (WF: rmap_wf mem rmap)
-        (VAL: val.(ValA.annot).(View.ts) <= List.length mem):
-    rmap_wf mem (RMap.add loc val rmap).
-  Proof.
-    inv WF. econs. i. unfold RMap.find, RMap.add. rewrite IdMap.add_spec.
-    condtac; viewtac.
-  Qed.
-
-  Lemma expr_wf
-        mem rmap e
-        (RMAP: rmap_wf mem rmap):
-    (sem_expr rmap e).(ValA.annot).(View.ts) <= List.length mem.
-  Proof.
-    induction e; viewtac. apply RMAP.
-  Qed.
-
-  Lemma read_wf
-        ts loc val mem
-        (READ: Memory.read loc ts mem = Some val):
-    ts <= List.length mem.
-  Proof.
-    revert READ. unfold Memory.read. destruct ts; [lia|]. s.
-    destruct (nth_error mem ts) eqn:NTH; ss. condtac; ss.
-    i. eapply List.nth_error_Some. congr.
-  Qed.
-
-  Lemma get_msg_wf
-        ts msg mem
-        (READ: Memory.get_msg ts mem = Some msg):
-    ts <= List.length mem.
-  Proof.
-    revert READ. unfold Memory.get_msg. destruct ts; [lia|]. s.
-    destruct (nth_error mem ts) eqn:NTH; ss. i. inv READ.
-    eapply List.nth_error_Some. congr.
-  Qed.
-
-  Lemma step0_wf tid e1 e2 eu1 eu2
-        (STEP: step0 tid e1 e2 eu1 eu2)
-        (EVENT: eqts_event e1 e2)
+  Lemma step0_wf tid e eu1 eu2
+        (STEP: step0 tid e e eu1 eu2)
         (WF: wf tid eu1):
     wf tid eu2.
   Proof.
-    destruct eu1 as [state1 local1 mem1].
-    destruct eu2 as [state2 local2 mem2].
-    inv WF. inv STEP. ss. subst.
+    admit.
+    (* destruct eu1 as [state1 local1 mem1]. *)
+    (* destruct eu2 as [state2 local2 mem2]. *)
+    (* inv WF. inv STEP. ss. subst. *)
 
-    assert (FWDVIEW: forall loc ts ord,
-               Memory.latest loc ts (View.ts (Local.coh local1 loc)) mem1 ->
-               ts <= length mem1 ->
-               View.ts (FwdItem.read_view (Local.fwdbank local1 loc) ts ord) <= length mem1).
-    { i. rewrite Local.fwd_read_view_le; eauto. }
-    generalize LOCAL. intro WF_LOCAL1.
-    inv STATE0; inv LOCAL0; inv EVENT; inv LOCAL; ss.
-    - econs; ss.
-      eauto using rmap_add_wf, expr_wf.
-    - inv RES. inv VIEW. inv VLOC. inv VIEW.
-      exploit Local.read_spec; eauto. intro READ_SPEC. guardH READ_SPEC.
-      inv STEP. ss. subst.
-      exploit FWDVIEW; eauto.
-      { eapply read_wf. eauto. }
-      i. econs; ss.
-      + apply rmap_add_wf; viewtac.
-        rewrite TS, <- TS0. viewtac.
-        eauto using expr_wf.
-      + econs; viewtac; eauto using expr_wf.
-        all: try by rewrite <- TS0; eauto using expr_wf.
-        * i. rewrite fun_add_spec. condtac; viewtac.
-          rewrite <- TS0. eauto using expr_wf.
-        * i. exploit FWDBANK; eauto. intro Y. inv Y. des.
-          econs; eauto. rewrite TS1, fun_add_spec. condtac; ss. inversion e. subst.
-          apply Memory.latest_ts_mon. apply join_l.
+    (* assert (FWDVIEW: forall loc ts ord, *)
+    (*            Memory.latest loc ts (View.ts (Local.coh local1 loc)) mem1 -> *)
+    (*            ts <= length mem1 -> *)
+    (*            View.ts (FwdItem.read_view (Local.fwdbank local1 loc) ts ord) <= length mem1). *)
+    (* { i. rewrite Local.fwd_read_view_le; eauto. } *)
+    (* generalize LOCAL. intro WF_LOCAL1. *)
+    (* inv STATE; inv LOCAL0; inv EVENT; inv LOCAL; ss. *)
+    (* - econs; ss. *)
+    (*   eauto using rmap_add_wf, expr_wf. *)
+    (* - inv RES. inv VIEW. inv VLOC. inv VIEW. *)
+    (*   exploit Local.read_spec; eauto. intro READ_SPEC. guardH READ_SPEC. *)
+    (*   inv STEP. ss. subst. *)
+    (*   exploit FWDVIEW; eauto. *)
+    (*   { eapply read_wf. eauto. } *)
+    (*   i. econs; ss. *)
+    (*   + apply rmap_add_wf; viewtac. *)
+    (*     rewrite TS, <- TS0. viewtac. *)
+    (*     eauto using expr_wf. *)
+    (*   + econs; viewtac; eauto using expr_wf. *)
+    (*     all: try by rewrite <- TS0; eauto using expr_wf. *)
+    (*     * i. rewrite fun_add_spec. condtac; viewtac. *)
+    (*       rewrite <- TS0. eauto using expr_wf. *)
+    (*     * i. exploit FWDBANK; eauto. intro Y. inv Y. des. *)
+    (*       econs; eauto. rewrite TS1, fun_add_spec. condtac; ss. inversion e. subst. *)
+    (*       apply Memory.latest_ts_mon. apply join_l. *)
     (* TODO: check *)
         (* * i. rewrite fun_add_spec in *. destruct ex0. *)
         (*   { inv H1. ss. condtac; [|congr]. econs; eauto. *)
@@ -595,8 +358,8 @@ Section ExecUnit.
         (*   } *)
         (* * i. eapply PROMISES0; eauto. eapply Time.le_lt_trans; [|by eauto]. *)
         (*   rewrite fun_add_spec. condtac; ss. inversion e. rewrite H2. apply join_l. *)
-    - inv RES. inv VIEW. inv VVAL. inv VIEW. inv VLOC. inv VIEW.
-      admit. (* promise_step_wf *)
+    (* - inv RES. inv VIEW. inv VVAL. inv VIEW. inv VLOC. inv VIEW. *)
+      (* admit. (* promise_step_wf *) *)
       (* inv STEP. inv WRITABLE. econs; ss. *)
       (* + apply rmap_add_wf; viewtac. *)
       (*   rewrite TS. unfold ifc. condtac; [|by apply bot_spec]. eapply get_msg_wf. eauto. *)
@@ -624,11 +387,11 @@ Section ExecUnit.
       (*     { eapply PROMISES0; eauto. revert TS2. condtac; ss. i. *)
       (*       inversion e. rewrite H2. rewrite COH0. ss. *)
       (*     } *)
-    - admit.
+    (* - admit. *)
       (* inv STEP. econs; ss. *)
     (* apply rmap_add_wf; viewtac. *)
     (* inv RES. inv VIEW. rewrite TS. s. apply bot_spec. *)
-    - inv STEP. econs; ss. econs; viewtac.
+    (* - inv STEP. econs; ss. econs; viewtac. *)
     (* - inv STEP. econs; ss. econs; viewtac. *)
     (* - inv LC. econs; ss. econs; viewtac. *)
     (*   inv CTRL. rewrite <- TS. eauto using expr_wf. *)
@@ -639,23 +402,7 @@ Section ExecUnit.
         (WF: wf tid eu1):
     wf tid eu2.
   Proof.
-    inv STEP. eapply step0_wf; eauto. refl.
-  Qed.
-
-  Lemma rmap_append_wf
-        mem msg rmap
-        (WF: rmap_wf mem rmap):
-    rmap_wf (mem ++ [msg]) rmap.
-  Proof.
-    inv WF. econs. i. rewrite RMAP. rewrite List.app_length. lia.
-  Qed.
-
-  Lemma rmap_interference_wf
-        mem rmap mem_interference
-        (WF: rmap_wf mem rmap):
-    rmap_wf (mem ++ mem_interference) rmap.
-  Proof.
-    inv WF. econs. i. rewrite RMAP, app_length. lia.
+    inv STEP. eapply step0_wf; eauto.
   Qed.
 
   (* TODO: move above.. *)
@@ -702,7 +449,7 @@ Section ExecUnit.
     - rewrite app_nil_r. ss.
   Qed.
   Next Obligation.
-    ii. inv H1. inv H2. econs; etrans; eauto.
+    ii. inv H. inv H0. econs; etrans; eauto.
     rewrite MEM, app_assoc. eauto.
   Qed.
 
@@ -719,7 +466,7 @@ End ExecUnit.
 
 Module Machine.
   Inductive t := mk {
-    tpool: IdMap.t (State.t (A:=View.t (A:=unit)) * Local.t (A:=unit));
+    tpool: IdMap.t (State.t (A:=unit) * Local.t);
     mem: Memory.t;
   }.
   Hint Constructors t.
@@ -737,7 +484,7 @@ Module Machine.
   .
   Hint Constructors is_terminal.
 
-  Inductive step (eustep: forall (tid:Id.t) (eu1 eu2:ExecUnit.t (A:=unit)), Prop) (m1 m2:t): Prop :=
+  Inductive step (eustep: forall (tid:Id.t) (eu1 eu2:ExecUnit.t), Prop) (m1 m2:t): Prop :=
   | step_intro
       tid st1 lc1 st2 lc2
       (FIND: IdMap.find tid m1.(tpool) = Some (st1, lc1))
@@ -785,8 +532,6 @@ Module Machine.
     econs. i. ss.
     rewrite IdMap.map_spec in FIND. destruct (IdMap.find tid p); inv FIND.
     econs; ss.
-    - econs. i. unfold RMap.find, RMap.init. rewrite IdMap.gempty. ss.
-    - apply Local.init_wf.
   Qed.
 
   Lemma step_step_wf
